First version of Mod_od with proof

num/Mod_op.v
@@ -1,26 +1,33 @@
 Set Implicit Arguments.
 
 Require Import ZArith.
+Require Import ZDivModAux.
 Require Import Basic_type.
 Require Import ZnZ.
 Require Import Zn2Z.
+Require Import Zn2Z_for_Proof.
+Require Import Zn2ZProof.
 
 Section Mod_op.
 
  Variable w : Set.
  
- Record mod_op : Set := mk_mod_op {
-   w0_mod    : w;
-   w1_mod    : w;
-   succ_mod  : w -> w;
-   add_mod   : w -> w -> w;
-   pred_mod  : w -> w;
-   sub_mod   : w -> w -> w;
-   mul_mod   : w -> w -> w;
+ Record mod_op : Set := mk_mod_op {    
+   w0_mod     : w;
+   w1_mod     : w;
+   succ_mod   : w -> w;
+   add_mod    : w -> w -> w;
+   pred_mod   : w -> w;
+   sub_mod    : w -> w -> w;
+   mul_mod    : w -> w -> w;
    square_mod : w -> w;
-   power_mod : w -> positive -> w
+   power_mod  : w -> positive -> w
+(*
+   shift      : w -> positive -> w;
+   trunc      : w -> positive -> w
+*)
  }.
- 
+
  Variable w_op : znz_op w.
  
  Let w_digits      := w_op.(znz_digits).
@@ -63,7 +70,7 @@ Section Mod_op.
  Let b2n := 
    match n with
    | N0 => b
-   | Npos p => w_add_mul_div b w0 p 
+   | Npos p => w_add_mul_div p b w0
    end.
 
  Let bm1 := w_sub b w1.
@@ -77,7 +84,7 @@ Section Mod_op.
    | N0 => fun ww => ww
    | Npos p => 
      let add_mul_div := ww_add_mul_div w_op in 
-     fun ww => add_mul_div ww W0 p
+     fun ww => add_mul_div p ww W0
    end.
 
  Let w_lsr_n :=
@@ -85,18 +92,226 @@ Section Mod_op.
    | N0 => fun w => w
    | Npos p =>
      let k := Pminus w_digits p in
-     fun w => w_add_mul_div w0 w k
+     fun w => w_add_mul_div k w0 w
    end.
+
+ Open Scope Z_scope. 
+ Notation "[| x |]" :=
+   (znz_to_Z w_op x)  (at level 0, x at level 99).
+
+Notation "[[ x ]]" :=
+   (ww_to_Z w_op x)  (at level 0, x at level 99).
+
+ Section Mod_spec.
+ 
+   Variable m_op : mod_op.
+
+   Variable wf: w -> Prop.
+
+   Record mod_spec : Set := mk_mod_spec {
+    (* Basic constructors *)
+      mod_wf_0          : wf w0;
+      mod_wf_spec_1     : wf w1;
+      succ_mod_wf_spec  : 
+                forall w, wf w -> wf (succ_mod m_op w);
+      add_mod_wf_spec   : 
+            forall w1 w2, wf w1 -> wf w2 -> wf (add_mod m_op w1 w2);
+      pred_mod_wf_spec  : 
+                forall w, wf w -> wf (pred_mod m_op w);
+      sub_mod_wf_spec   : 
+            forall w1 w2, wf w1 -> wf w2 -> wf (sub_mod m_op w1 w2);
+      mul_mod_wf_spec   : 
+            forall w1 w2, wf w1 -> wf w2 -> wf (mul_mod m_op w1 w2);
+      square_mod_wf_spec: 
+                forall w, wf w -> wf (square_mod m_op w);
+      power_mod_wf_spec : 
+              forall w p, wf w -> wf (power_mod m_op w p);
+(*
+      shift_wf_spec     :
+              forall w p, wf w -> wf (shift m_op w p);
+      trunc_wf_spec     :
+              forall w p, wf w -> wf (trunc m_op w p);
+*)
+      mod_spec_0        : [|w0|] mod [|b|] = 0;
+      mod_spec_1        : [|w1|] mod [|b|] = 1;
+      succ_mod_spec     : 
+                forall w, wf w ->
+                          [|succ_mod m_op w|] = ([|w|] + 1) mod [|b|];
+      add_mod_spec      :
+            forall w1 w2, wf w1 -> wf w2 ->
+                          [|add_mod m_op w1 w2|] = ([|w1|] + [|w2|]) mod [|b|];
+      pred_mod_spec     :
+                forall w, wf w ->
+                          [|pred_mod m_op w|] = ([|w|] - 1) mod [|b|];
+      sub_mod_spec      :
+            forall w1 w2, wf w1 -> wf w2 ->
+                          [|sub_mod m_op w1 w2|] = ([|w1|] - [|w2|]) mod [|b|];
+      mul_mod_spec      :
+            forall w1 w2, wf w1 -> wf w2 ->
+                          [|mul_mod m_op w1 w2|] = ([|w1|] * [|w2|]) mod [|b|];
+      square_mod_spec   :
+                forall w, wf w ->
+                          [|square_mod m_op w|] = ([|w|] * [|w|]) mod [|b|];
+      power_mod_spec    :
+              forall w p, wf w ->
+                          [|power_mod m_op w p|] = (Zpower_pos [|w|] p) mod [|b|]
+(*
+      shift_spec        :
+              forall w p, wf w -> 
+                          [|shift m_op w p|] = ([|w|] / (Zpower_pos 2 p)) mod [|b|];
+      trunc_spec        :
+              forall w p, wf w ->
+                          [|power_mod m_op w p|] = ([|w1|] mod (Zpower_pos 2 p)) mod [|b|]
+*)
+    }.
+
+  End Mod_spec.
+
+ Hypothesis b_pos: 1 < [|b|].
+
+ Lemma Zpower_n: 0 < 2 ^ Z_of_N n.
+ apply ZPowerAux.Zpower_lt_0; auto with zarith.
+ case n; intros; simpl Z_of_N; auto with zarith.
+ Qed.
+
+ Hint Resolve Zpower_n ZAux.Zmult_lt_0_compat ZPowerAux.Zpower_lt_0.
+ 
+ Let _wf := fun w => [|w|] < [|b|].
+
+ Variable op_spec: znz_spec w_op.
+
+ Variable m_op : mod_op.
+
+ Hint Rewrite 
+    (spec_0 op_spec)
+    (spec_1 op_spec)
+    (spec_Bm1 op_spec)
+    (spec_WW op_spec)
+    (spec_CW op_spec)
+    (spec_opp_c op_spec)
+    (spec_opp_carry op_spec)
+    (spec_succ_c op_spec)
+    (spec_add_c op_spec)
+    (spec_add_carry_c op_spec)
+    (spec_add op_spec)
+    (spec_pred_c op_spec)
+    (spec_sub_c op_spec)
+    (spec_sub_carry_c op_spec)
+    (spec_sub op_spec)
+    (spec_mul_c op_spec)
+    (spec_mul op_spec)
+    : w_rewrite.
 
  Let _w0_mod := w0.
 
+ Lemma _mod_wf_0: _wf _w0_mod.
+ unfold _w0_mod, _wf, w0.
+ autorewrite with w_rewrite; auto with zarith. 
+ Qed.
+
+ Lemma _mod_spec_0: [|_w0_mod|] mod [|b|] = 0.
+ rewrite Zmod_def_small;
+ unfold _w0_mod, w0; autorewrite with w_rewrite; auto with zarith. 
+ Qed.
+ 
  Let _w1_mod := w1.
 
+ Lemma _mod_wf_1: _wf _w1_mod.
+ unfold _w1_mod, _wf, w1.
+ autorewrite with w_rewrite; auto with zarith. 
+ Qed.
+
+ Lemma _mod_spec_1: [|_w1_mod|] mod [|b|] = 1.
+ rewrite Zmod_def_small;
+ unfold _w1_mod, w1; autorewrite with w_rewrite; auto with zarith. 
+ Qed.
+
  Let _succ_mod x :=
-  match w_compare x bm1 with 
-  | Lt => without_c (w_succ_c x)
+  let res := without_c (w_succ_c x) in
+  match w_compare res b with 
+  | Lt => res
   | _ => w0
   end.
+
+ Let _w0_is_0: [|w0|] = 0.
+ unfold znz_to_Z; rewrite <- (spec_0 op_spec); auto.
+ Qed.
+
+ Lemma _w0_wf : _wf w0.
+ unfold _wf; rewrite _w0_is_0; auto with zarith.
+ Qed.
+
+ Let _w1_is_1: [|w1|] = 1.
+ unfold znz_to_Z; rewrite <- (spec_1 op_spec); auto.
+ Qed.
+
+ Lemma _w1_wf : _wf w1.
+ unfold _wf; rewrite _w1_is_1; auto with zarith.
+ Qed.
+
+ Theorem Zmod_plus_one: forall a1 b1, 0 < b1 -> (a1 + b1) mod b1 = a1 mod b1.
+ intros a1 b1 H; rewrite Zmod_plus; auto with zarith.
+ rewrite Z_mod_same; try rewrite Zplus_0_r; auto with zarith.
+ apply Zmod_mod; auto.
+ Qed.
+
+ Theorem Zmod_minus_one: forall a1 b1, 0 < b1 -> (a1 - b1) mod b1 = a1 mod b1.
+ intros a1 b1 H; rewrite Zmod_minus; auto with zarith.
+ rewrite Z_mod_same; try rewrite Zminus_0_r; auto with zarith.
+ apply Zmod_mod; auto.
+ Qed.
+
+ Lemma _succ_mod_spec: forall w, _wf w ->
+    [|_succ_mod w|] = ([|w|] + 1) mod [|b|].
+ intros w2; unfold _wf, _succ_mod, w_compare; simpl.
+ match goal with |- context[znz_compare _ ?x ?y] =>
+   generalize (spec_compare op_spec x y);
+   case (znz_compare w_op x y); autorewrite with w_rewrite
+ end; try rewrite _w0_is_0; auto with zarith.
+ unfold without_c, w_succ_c.
+ generalize (spec_succ_c op_spec w2);  unfold interp_carry; 
+   case (znz_succ_c w_op w2).
+ intros w3 H H1 H2; rewrite <- H; rewrite H1.
+ apply sym_equal; apply Z_mod_same; auto with zarith.
+ rewrite Zmult_1_l; unfold base.
+ intros w3 H H1 H2.
+ absurd ([|b|] + 1 <= [|w2|] +1); auto with zarith.
+ rewrite <- H; rewrite <- H1; auto with zarith. 
+ rewrite (Zplus_comm [|w3|]); apply Zplus_le_compat_r.
+ replace 1 with (2 ^ 0); auto with zarith.
+ apply ZPowerAux.Zpower_le_monotone; auto with zarith.
+ unfold without_c, w_succ_c.
+ generalize (spec_succ_c op_spec w2);  unfold interp_carry; 
+   case (znz_succ_c w_op w2).
+ intros w3 H H1 H2; rewrite <- H.
+ apply sym_equal; apply Zmod_def_small; auto with zarith.
+ split; auto.
+ case (spec_to_Z op_spec w3); auto.
+ rewrite Zmult_1_l; unfold base.
+ intros w3 H H1 H2.
+ absurd ([|b|] + 1 <= [|w2|] +1); auto with zarith.
+ rewrite <- H; auto with zarith. 
+ apply Zle_trans with (2 ^ Zpos (znz_digits w_op)); auto with zarith.
+ case (spec_to_Z op_spec b); unfold base; auto with zarith.
+ case (spec_to_Z op_spec w3); unfold base; auto with zarith.
+ unfold without_c, w_succ_c.
+ generalize (spec_succ_c op_spec w2);  unfold interp_carry; 
+   case (znz_succ_c w_op w2).
+ intros w3 H H1 H2.
+ absurd ([|b|] + 1 <= [|w2|] +1); auto with zarith.
+ rewrite Zmult_1_l; unfold base.
+ intros w3 H H1 H2.
+ absurd ([|b|] + 1 <= [|w2|] +1); auto with zarith.
+ rewrite <- H; auto with zarith. 
+ apply Zle_trans with (2 ^ Zpos (znz_digits w_op)); auto with zarith.
+ case (spec_to_Z op_spec b); unfold base; auto with zarith.
+ Qed.
+
+
+ Lemma _succ_mod_wf_spec: forall w, _wf w -> _wf (_succ_mod w).
+ intros w2 Hw2; unfold _wf; rewrite _succ_mod_spec; auto.
+ case (Z_mod_lt ([|w2|] + 1) [|b|]); auto with zarith.
+ Qed.
 
  Let split := ww_split w_op.
 
@@ -111,17 +326,137 @@ Section Mod_op.
   | C1 z => w_add mb z
   end.
 
+ Lemma _add_mod_spec: forall w1 w2, _wf w1 -> _wf w2 ->
+     [|_add_mod w1 w2|] = ([|w1|] + [|w2|]) mod [|b|].
+ intros w2 w3; unfold _wf, _add_mod, w_compare, w_add_c; intros H H1.
+ match goal with |- context[znz_add_c _ ?x ?y] =>
+   generalize (spec_add_c op_spec x y); unfold interp_carry;
+   case (znz_add_c w_op x y); autorewrite with w_rewrite
+ end; auto with zarith.
+ intros w4 H2.
+ match goal with |- context[znz_compare _ ?x ?y] =>
+   generalize (spec_compare op_spec x y); unfold interp_carry;
+   case (znz_compare w_op x y); autorewrite with w_rewrite
+ end; auto with zarith.
+ intros H3; rewrite <- H2; rewrite H3.
+ rewrite Z_mod_same; auto with zarith.
+ intros H3; rewrite <- H2.
+ apply sym_equal; apply Zmod_def_small; auto with zarith.
+ case (spec_to_Z op_spec w4); unfold base; auto with zarith.
+ intros H3.
+ rewrite <- H2.
+ assert (F1: 0 < [|w4|] - [|b|]); auto with zarith.
+ assert (F2: [|w4|] < [|b|] + [|b|]); auto with zarith.
+ rewrite (fun x y => Zmod_def_small (x - y)); auto with zarith.
+ rewrite <- (Zmod_minus_one [|w4|]); auto with zarith.
+ apply sym_equal; apply Zmod_def_small; auto with zarith.
+ split; auto with zarith.
+ apply Zlt_trans with [|b|]; auto with zarith.
+ case (spec_to_Z op_spec b); unfold base; auto with zarith.
+ rewrite Zmult_1_l; intros w4 H2; rewrite <- H2.
+ unfold mb, w_add; rewrite spec_add; auto with zarith.
+ unfold without_c, w_opp_c.
+ assert (F1: [|w4|] < [|b|]).
+ assert (F2: base (znz_digits w_op) + [|w4|] < base (znz_digits w_op) + [|b|]);
+   auto with zarith.
+ case (spec_to_Z op_spec w2); auto with zarith.
+ assert (F2: [|b|] < base (znz_digits w_op) + [|w4|]); auto with zarith.
+ apply Zlt_le_trans with (base (znz_digits w_op)); auto with zarith.
+ case (spec_to_Z op_spec b); auto with zarith.
+ case (spec_to_Z op_spec w4); auto with zarith.
+ assert (F3: base (znz_digits w_op) + [|w4|] < [|b|] + [|b|]); auto with zarith.
+ rewrite <- (fun x => Zmod_minus_one (base x + [|w4|])); auto with zarith.
+ rewrite (fun x y => Zmod_def_small (x - y)); auto with zarith.
+ match goal with |- context[znz_opp_c _ ?x] =>
+   generalize (spec_opp_c op_spec x); unfold interp_carry;
+   case (znz_opp_c w_op x); autorewrite with w_rewrite
+ end; auto with zarith.
+ intros w5 H3; rewrite H3.
+ rewrite <- (fun x => Zmod_plus_one (-x + [|w4|])); auto with zarith.
+ rewrite Zmod_def_small; auto with zarith.
+ intros w5 H3.
+ replace [|w5|] with (base (znz_digits w_op) - [|b|]); auto with zarith.
+ rewrite Zmod_def_small; auto with zarith.
+ Qed.
+
+ Lemma _add_mod_wf_spec: forall w1 w2, _wf w1 -> _wf w2 -> _wf (_add_mod w1 w2).
+ intros w2 w3 H H1.
+ unfold _wf; rewrite _add_mod_spec; auto.
+ case (Z_mod_lt ([|w2|] + [|w3|]) [|b|]); auto with zarith.
+ Qed.
+
  Let _pred_mod x :=
   match w_compare w0 x with
   | Eq => bm1
   | _ => without_c (w_pred_c x)
   end.
 
+ Lemma _pred_mod_spec: forall w, _wf w ->
+   [|_pred_mod w|] = ([|w|] - 1) mod [|b|].
+ intros w2; unfold _wf, _pred_mod, w_compare, bm1; simpl.
+ match goal with |- context[znz_compare _ ?x ?y] =>
+   generalize (spec_compare op_spec x y);
+   case (znz_compare w_op x y); autorewrite with w_rewrite
+ end; try rewrite _w0_is_0; try rewrite _w1_is_1; auto with zarith.
+ intros H H1; rewrite <- H; simpl.
+ rewrite <- (Zmod_plus_one (-1)); auto with zarith.
+ repeat rewrite Zmod_def_small; auto with zarith.
+ case (spec_to_Z op_spec b); auto with zarith.
+ intros H1 H2. 
+ unfold without_c, w_pred_c.
+ generalize (spec_pred_c op_spec w2);  unfold interp_carry; 
+   case (znz_pred_c w_op w2).
+ intros w3 H3; rewrite H3.
+ apply sym_equal; apply Zmod_def_small; auto with zarith.
+ intros w3 H3.
+ absurd (0 <= [|w2|] -1); auto with zarith.
+ rewrite <- H3; auto with zarith. 
+ case (spec_to_Z op_spec w3); auto with zarith.
+ case (spec_to_Z op_spec w2); auto with zarith.
+ Qed.
+
+ Lemma _pred_mod_wf_spec: forall w, _wf w -> _wf (_pred_mod w).
+ intros w2 Hw2; unfold _wf; rewrite _pred_mod_spec; auto.
+ case (Z_mod_lt ([|w2|] - 1) [|b|]); auto with zarith.
+ Qed.
+
  Let _sub_mod x y :=
   match w_sub_c x y with
   | C0 z => z
   | C1 z => w_add z b
   end.
+
+ Lemma _sub_mod_spec: forall w1 w2, _wf w1 -> _wf w2 ->
+   [|_sub_mod w1 w2|] = ([|w1|] - [|w2|]) mod [|b|].
+ intros w2 w3; unfold _wf, _sub_mod, w_compare, w_sub_c; intros H H1.
+ match goal with |- context[znz_sub_c _ ?x ?y] =>
+   generalize (spec_sub_c op_spec x y); unfold interp_carry;
+   case (znz_sub_c w_op x y); autorewrite with w_rewrite
+ end; auto with zarith.
+ intros w4 H2.
+ rewrite Zmod_def_small; auto with zarith.
+ split; auto with zarith.
+ rewrite <- H2; case (spec_to_Z op_spec w4); auto with zarith.
+ apply Zle_lt_trans with [|w2|]; auto with zarith.
+ case (spec_to_Z op_spec w3); auto with zarith.
+ intros w4 H2; rewrite <- H2.
+ unfold w_add; rewrite spec_add; auto with zarith.
+ case (spec_to_Z op_spec w4); intros F1 F2.
+ assert (F3: 0 <= - 1 *  base (znz_digits w_op) + [|w4|] + [|b|]); auto with zarith.
+ rewrite H2.
+ case (spec_to_Z op_spec w3); case (spec_to_Z op_spec w2); auto with zarith.
+ rewrite <- (fun x => Zmod_minus_one ([|w4|] + x)); auto with zarith.
+ rewrite <- (fun x y => Zmod_plus_one (-y + x)); auto with zarith.
+ repeat rewrite Zmod_def_small; auto with zarith.
+ case (spec_to_Z op_spec b); auto with zarith.
+ Qed.
+
+ Lemma _sub_mod_wf_spec: forall w1 w2, _wf w1 -> _wf w2 ->
+   _wf (_sub_mod w1 w2).
+ intros w2 w3 H H1.
+ unfold _wf; rewrite _sub_mod_spec; auto.
+ case (Z_mod_lt ([|w2|] - [|w3|]) [|b|]); auto with zarith.
+ Qed.
 
  Let _mul_mod x y :=
   let xy := w_mul_c x y in
@@ -135,6 +470,288 @@ Section Mod_op.
     w_lsr_n r 
   end.
 
+ Theorem n_spec: base (znz_digits w_op) / 2 <= 2 ^ (Z_of_N n) * [|b|] 
+                        < base (znz_digits w_op).
+ unfold n, w_head0; apply (spec_head0 op_spec); auto with zarith.
+ Qed. 
+
+ Theorem b2n_spec: [|b2n|] = 2 ^ (Z_of_N n) * [|b|].
+ unfold b2n, w_add_mul_div; generalize n_spec; case n; auto.
+ simpl Z_of_N; rewrite ZPowerAux.Zpower_exp_0; auto with zarith.
+ intros p (Hp, Hp1).
+ assert (F1: Zpos p < Zpos (znz_digits w_op)).
+ case (Zle_or_lt (Zpos (znz_digits w_op)) (Zpos p)); auto with zarith.
+ intros H1; contradict Hp1; apply Zle_not_lt; unfold base.
+ apply Zle_trans with (2 ^ Zpos p * 1); auto with zarith.
+ rewrite Zmult_1_r; apply ZPowerAux.Zpower_le_monotone; auto with zarith.
+ rewrite (spec_add_mul_div op_spec); auto with zarith.
+ rewrite _w0_is_0; rewrite Zdiv_0; auto with zarith.
+ rewrite Zplus_0_r; rewrite Zmult_comm; apply Zmod_def_small; auto with zarith.
+ split; auto with zarith; red; auto.
+ Qed.
+
+ Theorem ww_lsl_n_spec: forall w, [[w]] < [|b|] * [|b|] ->
+   [[ww_lsl_n w]] = 2 ^ (Z_of_N n) * [[w]].
+ intros w2 H; unfold ww_lsl_n; generalize n_spec; case n; simpl Z_of_N.
+ intros _; rewrite ZPowerAux.Zpower_exp_0; auto with zarith.
+ intros p (Hp, Hp1).
+ assert (F: forall x, 0 < Zpos x); auto with zarith.
+ intros x; red; simpl; auto.
+ assert (F0: forall x, 2 * x = x + x); auto with zarith.
+ assert (F1: Zpos p < Zpos (znz_digits w_op)).
+ case (Zle_or_lt (Zpos (znz_digits w_op)) (Zpos p)); auto.
+ intros H1; contradict Hp1; apply Zle_not_lt; unfold base.
+ apply Zle_trans with (2 ^ Zpos p * 1); auto with zarith.
+ rewrite Zmult_1_r; apply ZPowerAux.Zpower_le_monotone; auto with zarith.
+ assert (F2: Zpos p < Zpos (xO (znz_digits w_op))).
+ rewrite (Zpos_xO (znz_digits w_op)); rewrite F0; auto with zarith.
+ pattern (Zpos p); rewrite <- Zplus_0_r; auto with zarith.
+ apply Zplus_lt_compat; auto with zarith.
+ rewrite (spec_ww_add_mul_div op_spec); auto with zarith.
+ rewrite spec_ww_0; rewrite Zdiv_0; auto with zarith.
+ rewrite Zplus_0_r; rewrite Zmod_def_small; auto with zarith.
+ split; auto with zarith.
+ case (spec_ww_to_Z op_spec w2); auto with zarith.
+ apply Zlt_trans with ([|b|] * [|b|] * 2 ^ Zpos p); auto with zarith.
+ apply Zmult_lt_compat_r; auto with zarith.
+ rewrite <- Zmult_assoc.
+ unfold base; unfold base in Hp.
+ rewrite (Zpos_xO (znz_digits w_op)); rewrite F0; auto with zarith.
+ rewrite Zpower_exp; auto with zarith.
+ apply ZAux.Zmult_lt_compat; auto with zarith.
+ case (spec_to_Z op_spec b); auto with zarith.
+ split; auto with zarith.
+ rewrite Zmult_comm; auto with zarith.
+ Qed.
+
+ Theorem w_lsr_n_spec: forall w, [|w|] < 2 ^ (Z_of_N n) *  [|b|]->
+   [|w_lsr_n w|] = [|w|] / 2 ^ (Z_of_N n).
+ intros w2 H.
+ assert (F: forall x, 0 < Zpos x); auto with zarith.
+ intros x; red; simpl; auto.
+ case (spec_to_Z op_spec w2); intros U1 U2.
+ unfold w_lsr_n; generalize n_spec; case n; simpl Z_of_N.
+ intros _; rewrite ZPowerAux.Zpower_exp_0; auto with zarith.
+ pattern [|w2|] at 2; rewrite <- Zmult_1_r; rewrite Z_div_mult; auto with zarith.
+ intros p (Hp, Hp1).
+ assert (F0: forall x, 2 * x = x + x); auto with zarith.
+ assert (F1: Zpos p < Zpos (znz_digits w_op)).
+ case (Zle_or_lt (Zpos (znz_digits w_op)) (Zpos p)); auto.
+ intros H1; contradict Hp1; apply Zle_not_lt; unfold base.
+ apply Zle_trans with (2 ^ Zpos p * 1); auto with zarith.
+ rewrite Zmult_1_r; apply ZPowerAux.Zpower_le_monotone; auto with zarith.
+ rewrite (spec_add_mul_div op_spec); auto with zarith.
+ rewrite _w0_is_0; rewrite Zmult_0_l; auto with zarith.
+ rewrite Zplus_0_l; rewrite Zpos_minus; auto with zarith.
+ replace (Zpos (znz_digits w_op) - (Zpos w_digits - Zpos p)) with
+   (Zpos p); auto with zarith.
+ 2: unfold w_digits; auto with zarith.
+ apply Zmod_def_small; auto with zarith.
+ split; auto with zarith.
+ case Zle_lt_or_eq with (1 := U1); intros U3; subst.
+ apply Zlt_trans with [|w2|]; auto with zarith.
+ apply Z_div_lt; auto with zarith.
+ apply Zle_ge; pattern 2 at 1; rewrite <- ZPowerAux.Zpower_exp_1; auto with zarith.
+ apply ZPowerAux.Zpower_le_monotone; auto with zarith.
+ split; auto with zarith.
+ case p; intros; red; simpl; auto; intros; discriminate.
+ rewrite <- U3; rewrite Zdiv_0; auto with zarith.
+ split; auto with zarith.
+ unfold w_digits; rewrite Zpos_minus; auto with zarith.
+ generalize (F p); auto with zarith.
+ Qed.
+
+ Lemma _mul_mod_spec: forall w1 w2, _wf w1 -> _wf w2 ->
+   [|_mul_mod w1 w2|] = ([|w1|] * [|w2|]) mod [|b|].
+ intros w2 w3; unfold _wf, _mul_mod, ww_compare, wwb, w_mul_c; intros H H1.
+ match goal with |- context[znz_mul_c _ ?x ?y] =>
+   generalize (spec_mul_c op_spec x y); unfold interp_carry;
+   case (znz_mul_c w_op x y); autorewrite with w_rewrite
+ end; auto with zarith.
+ match goal with |- context[znz_compare _ ?x ?y] =>
+   generalize (spec_compare op_spec x y);
+   case (znz_compare w_op x y); autorewrite with w_rewrite
+ end; try rewrite _w0_is_0; try rewrite _w1_is_1; auto with zarith.
+ match goal with |- context[znz_compare
+ _ ?x ?y] =>
+   generalize (spec_compare op_spec x y);
+   case (znz_compare w_op x y); autorewrite with w_rewrite
+ end; try rewrite _w0_is_0; try rewrite _w1_is_1; auto with zarith.
+ intros H2 H3 H4; rewrite <- H4.
+ simpl; rewrite (spec_0 op_spec).
+ rewrite Zmod_def_small; auto with zarith.
+ simpl; intros w4 s5 H2.
+ match goal with |- context[znz_compare _ ?x ?y] =>
+   generalize (spec_compare op_spec x y);
+   case (znz_compare w_op x y); autorewrite with w_rewrite
+ end; try rewrite _w0_is_0; try rewrite _w1_is_1; auto with zarith.
+ intros H3; rewrite <- H2; rewrite H3; simpl.
+ match goal with |- context[znz_compare _ ?x ?y] =>
+   generalize (spec_compare op_spec x y);
+   case (znz_compare w_op x y); autorewrite with w_rewrite
+ end; try rewrite _w0_is_0; try rewrite _w1_is_1; auto with zarith.
+ intros H4; rewrite H4; rewrite Z_mod_same; auto with zarith.
+ intros H4; rewrite Zmod_def_small; auto with zarith.
+ case (spec_to_Z op_spec s5); auto with zarith.
+ rewrite H3 in H2; simpl in H2.
+ generalize (ww_lsl_n_spec (WW w4 s5)); 
+  case (ww_lsl_n (WW w4 s5)); auto with arith.
+ simpl; rewrite H3; rewrite H2; simpl.
+ intros H4 H5; contradict H5; apply Zle_not_gt.
+ apply Zmult_le_reg_r with (2 ^ Z_of_N n); auto with zarith.
+ rewrite Zmult_comm; rewrite <- H4; auto with zarith.
+ apply ZAux.Zmult_lt_compat_bis.
+ case (spec_to_Z op_spec w2); auto with zarith.
+ case (spec_to_Z op_spec w3); auto with zarith.
+ simpl; rewrite H3; rewrite Zmult_0_l; rewrite Zplus_0_l.
+ intros w5 w6; simpl; intros H4 H5.
+ match type of H4 with ?X -> ?Y =>
+   assert (tmp: X); 
+    [idtac | generalize (H4 tmp); clear tmp H4; intros H4]
+ end.
+ rewrite H2; apply ZAux.Zmult_lt_compat_bis.
+ case (spec_to_Z op_spec w2); auto with zarith.
+ case (spec_to_Z op_spec w3); auto with zarith.
+ unfold w_div21; generalize (spec_div21 op_spec w5 w6 b2n);
+   case (znz_div21 w_op w5 w6 b2n).
+ intros w7 w8 H6; case H6.
+ rewrite b2n_spec; case (n_spec); auto.
+ rewrite b2n_spec.
+ case (Zle_or_lt (2 ^ Z_of_N n * [|b|]) [|w5|]); auto; intros H7.
+ match type of H4 with ?X = ?Y =>
+    absurd (Y < X)
+ end.
+ apply Zle_not_lt; rewrite H4; auto with zarith.
+ rewrite H2.
+ match goal with |- ?X < ?Y + _ =>
+    apply Zlt_le_trans with Y; auto with zarith
+ end.
+ rewrite Zmult_assoc; match goal with |- ?X * ?Y < _ =>
+    apply Zle_lt_trans with ([|w5|] * Y); auto with zarith
+ end.
+ apply Zmult_le_compat_r; auto with zarith.
+ case (spec_to_Z op_spec w3); auto with zarith.
+ apply Zmult_lt_compat_l; auto with zarith.
+ apply Zlt_le_trans with (2 := H7); auto with zarith.
+ apply Zlt_trans with [|b|]; auto with zarith.
+ case (spec_to_Z op_spec b); auto with zarith.
+ case (spec_to_Z op_spec w6); auto with zarith.
+ clear H6; rewrite b2n_spec; auto with zarith; intros H6 H7.
+ rewrite w_lsr_n_spec; auto with zarith.
+ rewrite H6 in H4.
+ match type of H4 with ?X * (?Y * ?Z) + ?T = ?Y * ?U =>
+   replace T with (Y * (U - X * Z))
+ end; auto with zarith.
+ rewrite Zmult_comm; rewrite Z_div_mult; auto with zarith.           
+ match goal with |- ?X - ?Y = ?X mod ?T =>
+  apply trans_equal with (((X - Y) + Y) mod T)
+ end.
+ rewrite Z_mod_plus; auto with zarith.
+ apply sym_equal; apply Zmod_def_small; auto with zarith.
+ split; auto with zarith.
+ apply Zmult_le_reg_r with (2 ^ Z_of_N n); auto with zarith.
+ rewrite Zmult_0_l; rewrite Zmult_comm.
+ rewrite Zmult_minus_distr_l.
+ rewrite <- H4; auto with zarith.
+ match goal with |- 0 <= ?X =>
+  replace X with [|w8|]; auto with zarith
+ end; ring.
+ apply Zmult_lt_reg_r with (2 ^ Z_of_N n); auto with zarith.
+ repeat rewrite (fun x y => Zmult_comm x (2 ^y)).
+ rewrite Zmult_minus_distr_l.
+ rewrite <- H4; auto with zarith.
+ match goal with |- ?X < _ =>
+  replace X with [|w8|]; auto with zarith
+ end; ring.
+ eq_tac; auto with zarith.
+ rewrite Zmult_minus_distr_l; rewrite <- H4; auto with zarith.
+ ring.
+ case (spec_to_Z op_spec w4); auto with zarith.
+ intros H3.
+ assert (F0: [[WW w4 s5]] < [|b|] * [|b|]).
+ simpl; rewrite H2; apply ZAux.Zmult_lt_compat_bis.
+ case (spec_to_Z op_spec w2); auto with zarith.
+ case (spec_to_Z op_spec w3); auto with zarith.
+ generalize (ww_lsl_n_spec (WW w4 s5) F0); clear F0;
+  case (ww_lsl_n (WW w4 s5)); auto with arith.
+ simpl.
+ intros HH.
+ match type of HH with ?Y = ?Z =>
+    absurd (Y < Z)
+ end.
+ rewrite <- HH; auto with zarith.
+ apply ZAux.Zmult_lt_0_compat; auto with zarith.
+ match goal with |- ?X < ?Y + ?Z =>
+    apply Zlt_le_trans with Y; auto with zarith
+ end.
+ apply ZAux.Zmult_lt_0_compat; auto with zarith.
+ unfold base; apply ZPowerAux.Zpower_lt_0; auto with zarith.
+ case (spec_to_Z op_spec s5); auto with zarith.
+ intros w5 w6; simpl; intros H4.
+ unfold w_div21; generalize (spec_div21 op_spec w5 w6 b2n);
+   case (znz_div21 w_op w5 w6 b2n).
+ intros w7 w8 H6; case H6.
+ rewrite b2n_spec; case (n_spec); auto.
+ rewrite b2n_spec.
+ case (Zle_or_lt (2 ^ Z_of_N n * [|b|]) [|w5|]); auto; intros H7.
+ match type of H4 with ?X = ?Y =>
+    absurd (Y < X)
+ end.
+ apply Zle_not_lt; rewrite H4; auto with zarith.
+ rewrite H2.
+ match goal with |- ?X < ?Y + _ =>
+    apply Zlt_le_trans with Y; auto with zarith
+ end.
+ rewrite Zmult_assoc; match goal with |- ?X * ?Y < _ =>
+    apply Zle_lt_trans with ([|w5|] * Y); auto with zarith
+ end.
+ apply Zmult_le_compat_r; auto with zarith.
+ case (spec_to_Z op_spec w3); auto with zarith.
+ apply Zmult_lt_compat_l; auto with zarith.
+ apply Zlt_le_trans with (2 := H7); auto with zarith.
+ apply Zlt_trans with [|b|]; auto with zarith.
+ case (spec_to_Z op_spec b); auto with zarith.
+ case (spec_to_Z op_spec w6); auto with zarith.
+ clear H6; rewrite b2n_spec; auto with zarith; intros H6 H7.
+ rewrite w_lsr_n_spec; auto with zarith.
+ rewrite H6 in H4.
+ match type of H4 with ?X * (?Y * ?Z) + ?T = ?Y * ?U =>
+   replace T with (Y * (U - X * Z))
+ end; auto with zarith.
+ rewrite Zmult_comm; rewrite Z_div_mult; auto with zarith.           
+ rewrite <- H2;
+ match goal with |- ?X - ?Y = ?X mod ?T =>
+  apply trans_equal with (((X - Y) + Y) mod T)
+ end.
+ rewrite Z_mod_plus; auto with zarith.
+ apply sym_equal; apply Zmod_def_small; auto with zarith.
+ split; auto.
+ apply Zmult_le_reg_r with (2 ^ Z_of_N n); auto with zarith.
+ rewrite Zmult_0_l; rewrite Zmult_comm.
+ rewrite Zmult_minus_distr_l.
+ rewrite <- H4; auto with zarith.
+ match goal with |- 0 <= ?X =>
+  replace X with [|w8|]; auto with zarith
+ end; ring.
+ apply Zmult_lt_reg_r with (2 ^ Z_of_N n); auto with zarith.
+ repeat rewrite (fun x y => Zmult_comm x (2 ^y)).
+ rewrite Zmult_minus_distr_l.
+ rewrite <- H4; auto with zarith.
+ match goal with |- ?X < _ =>
+  replace X with [|w8|]; auto with zarith
+ end; ring.
+ eq_tac; auto with zarith.
+ rewrite Zmult_minus_distr_l; rewrite <- H4; auto with zarith.
+ ring.
+ Qed.
+
+ Lemma _mul_mod_wf_spec: forall w1 w2, _wf w1 -> _wf w2 ->
+   _wf (_mul_mod w1 w2).
+ intros w2 w3 H H1.
+ unfold _wf; rewrite _mul_mod_spec; auto.
+ case (Z_mod_lt ([|w2|] * [|w3|]) [|b|]); auto with zarith.
+ Qed.
+
  Let _square_mod x :=
   let x2 := w_square_c x in
   match ww_compare w_op x2 wwb with
@@ -147,7 +764,186 @@ Section Mod_op.
     w_lsr_n r
   end.
 
-  Let _power_mod :=
+ Lemma _square_mod_spec: forall w, _wf w ->
+    [|_square_mod w|] = ([|w|] * [|w|]) mod [|b|].
+ intros w2; unfold _wf, _square_mod, ww_compare, w_square_c.
+ match goal with |- context[znz_square_c _ ?x] =>
+   generalize (spec_square_c op_spec x); unfold interp_carry;
+   case (znz_square_c w_op x); autorewrite with w_rewrite
+ end; auto with zarith.
+ simpl.
+ match goal with |- context[znz_compare _ ?x ?y] =>
+   generalize (spec_compare op_spec x y);
+   case (znz_compare w_op x y); autorewrite with w_rewrite
+ end; try rewrite _w0_is_0; try rewrite _w1_is_1; auto with zarith.
+ match goal with |- context[znz_compare
+ _ ?x ?y] =>
+   generalize (spec_compare op_spec x y);
+   case (znz_compare w_op x y); autorewrite with w_rewrite
+ end; try rewrite _w0_is_0; try rewrite _w1_is_1; auto with zarith.
+ intros H2 H3 H4 _; rewrite <- H4.
+ rewrite Zmod_def_small; auto with zarith.
+ simpl; intros w3 s4 H2.
+ match goal with |- context[znz_compare _ ?x ?y] =>
+   generalize (spec_compare op_spec x y);
+   case (znz_compare w_op x y); autorewrite with w_rewrite
+ end; try rewrite _w0_is_0; try rewrite _w1_is_1; auto with zarith.
+ intros H3; rewrite <- H2; rewrite H3; simpl.
+ match goal with |- context[znz_compare _ ?x ?y] =>
+   generalize (spec_compare op_spec x y);
+   case (znz_compare w_op x y); autorewrite with w_rewrite
+ end; try rewrite _w0_is_0; try rewrite _w1_is_1; auto with zarith.
+ intros H4 _; rewrite H4.
+ rewrite Z_mod_same; auto with zarith.
+ intros H4 _; rewrite Zmod_def_small; auto with zarith.
+ case (spec_to_Z op_spec s4); auto with zarith.
+ rewrite H3 in H2; simpl in H2.
+ intros H4 H5.
+ assert (F0: [[WW w3 s4]] < [|b|] * [|b|]).
+ simpl; rewrite H3; simpl; rewrite H2.
+ apply ZAux.Zmult_lt_compat_bis.
+ case (spec_to_Z op_spec w2); auto with zarith.
+ case (spec_to_Z op_spec w2); auto with zarith.
+ generalize (ww_lsl_n_spec (WW w3 s4) F0); clear F0;
+  case (ww_lsl_n (WW w3 s4)); auto with arith.
+ simpl; rewrite H3; rewrite H2; simpl; rewrite H2 in H4.
+ intros H6; contradict H4; apply Zle_not_gt.
+ apply Zmult_le_reg_r with (2 ^ Z_of_N n); auto with zarith.
+ rewrite Zmult_comm; rewrite <- H6; auto with zarith.
+ simpl; rewrite H3; rewrite Zmult_0_l; rewrite Zplus_0_l.
+ intros w4 w5; simpl; intros H6.
+ unfold w_div21; generalize (spec_div21 op_spec w4 w5 b2n);
+   case (znz_div21 w_op w4 w5 b2n).
+ intros w6 w7 H7; case H7; clear H7.
+ rewrite b2n_spec; case (n_spec); auto.
+ rewrite b2n_spec.
+ apply Zmult_lt_reg_r with (base (znz_digits w_op)); auto with zarith.
+ unfold base; auto with zarith.
+ match type of H6 with ?X = _ =>
+   apply Zle_lt_trans with X
+ end; auto with zarith.
+ case (spec_to_Z op_spec w5); auto with zarith.
+ rewrite H6. 
+ rewrite <- Zmult_assoc; apply Zmult_lt_compat_l; auto with zarith.
+ simpl; rewrite H2; apply ZAux.Zmult_lt_compat_bis.
+ case (spec_to_Z op_spec w2); auto with zarith.
+ case (spec_to_Z op_spec w2); auto with zarith.
+ rewrite b2n_spec; auto with zarith; intros H7 H8.
+ rewrite w_lsr_n_spec; auto with zarith.
+ rewrite H7 in H6.
+ match type of H6 with ?X * (?Y * ?Z) + ?T = ?Y * ?U =>
+   replace T with (Y * (U - X * Z))
+ end; auto with zarith.
+ rewrite Zmult_comm; rewrite Z_div_mult; auto with zarith.           
+ match goal with |- ?X - ?Y = ?X mod ?T =>
+  apply trans_equal with (((X - Y) + Y) mod T)
+ end.
+ rewrite Z_mod_plus; auto with zarith.
+ apply sym_equal; apply Zmod_def_small; auto with zarith.
+ split; auto with zarith.
+ apply Zmult_le_reg_r with (2 ^ Z_of_N n); auto with zarith.
+ rewrite Zmult_0_l; rewrite Zmult_comm.
+ rewrite Zmult_minus_distr_l.
+ rewrite <- H6; auto with zarith.
+ match goal with |- 0 <= ?X =>
+  replace X with [|w7|]; auto with zarith
+ end; ring.
+ apply Zmult_lt_reg_r with (2 ^ Z_of_N n); auto with zarith.
+ repeat rewrite (fun x y => Zmult_comm x (2 ^y)).
+ rewrite Zmult_minus_distr_l.
+ rewrite <- H6; auto with zarith.
+ match goal with |- ?X < _ =>
+  replace X with [|w7|]; auto with zarith
+ end; ring.
+ eq_tac; auto with zarith.
+ rewrite Zmult_minus_distr_l; rewrite <- H6; auto with zarith.
+ ring.
+ case (spec_to_Z op_spec w3); auto with zarith.
+ intros H3 H4.
+ assert (F0: [[WW w3 s4]] < [|b|] * [|b|]).
+ simpl; rewrite H2; apply ZAux.Zmult_lt_compat_bis.
+ case (spec_to_Z op_spec w2); auto with zarith.
+ case (spec_to_Z op_spec w2); auto with zarith.
+ generalize (ww_lsl_n_spec (WW w3 s4) F0); clear F0;
+  case (ww_lsl_n (WW w3 s4)); auto with arith.
+ simpl.
+ intros HH.
+ match type of HH with ?Y = ?Z =>
+    absurd (Y < Z)
+ end.
+ rewrite <- HH; auto with zarith.
+ apply ZAux.Zmult_lt_0_compat; auto with zarith.
+ match goal with |- ?X < ?Y + ?Z =>
+    apply Zlt_le_trans with Y; auto with zarith
+ end.
+ apply ZAux.Zmult_lt_0_compat; auto with zarith.
+ unfold base; apply ZPowerAux.Zpower_lt_0; auto with zarith.
+ case (spec_to_Z op_spec s4); auto with zarith.
+ intros w4 w5; simpl; intros H5.
+ unfold w_div21; generalize (spec_div21 op_spec w4 w5 b2n);
+   case (znz_div21 w_op w4 w5 b2n).
+ intros w6 w7 H6; case H6.
+ rewrite b2n_spec; case (n_spec); auto.
+ rewrite b2n_spec.
+ case (Zle_or_lt (2 ^ Z_of_N n * [|b|]) [|w4|]); auto; intros H7.
+ match type of H5 with ?X = ?Y =>
+    absurd (Y < X)
+ end.
+ apply Zle_not_lt; rewrite H5; auto with zarith.
+ rewrite H2.
+ match goal with |- ?X < ?Y + _ =>
+    apply Zlt_le_trans with Y; auto with zarith
+ end.
+ rewrite Zmult_assoc; match goal with |- ?X * ?Y < _ =>
+    apply Zle_lt_trans with ([|w4|] * Y); auto with zarith
+ end.
+ apply Zmult_le_compat_r; auto with zarith.
+ case (spec_to_Z op_spec w2); auto with zarith.
+ apply Zmult_lt_compat_l; auto with zarith.
+ apply Zlt_le_trans with (2 := H7); auto with zarith.
+ case (spec_to_Z op_spec w2); auto with zarith.
+ case (spec_to_Z op_spec w5); auto with zarith.
+ clear H6; rewrite b2n_spec; auto with zarith; intros H6 H7.
+ rewrite w_lsr_n_spec; auto with zarith.
+ rewrite H6 in H5.
+ match type of H5 with ?X * (?Y * ?Z) + ?T = ?Y * ?U =>
+   replace T with (Y * (U - X * Z))
+ end; auto with zarith.
+ rewrite Zmult_comm; rewrite Z_div_mult; auto with zarith.           
+ rewrite <- H2;
+ match goal with |- ?X - ?Y = ?X mod ?T =>
+  apply trans_equal with (((X - Y) + Y) mod T)
+ end.
+ rewrite Z_mod_plus; auto with zarith.
+ apply sym_equal; apply Zmod_def_small; auto with zarith.
+ split; auto.
+ apply Zmult_le_reg_r with (2 ^ Z_of_N n); auto with zarith.
+ rewrite Zmult_0_l; rewrite Zmult_comm.
+ rewrite Zmult_minus_distr_l.
+ rewrite <- H5; auto with zarith.
+ match goal with |- 0 <= ?X =>
+  replace X with [|w7|]; auto with zarith
+ end; ring.
+ apply Zmult_lt_reg_r with (2 ^ Z_of_N n); auto with zarith.
+ repeat rewrite (fun x y => Zmult_comm x (2 ^y)).
+ rewrite Zmult_minus_distr_l.
+ rewrite <- H5; auto with zarith.
+ match goal with |- ?X < _ =>
+  replace X with [|w7|]; auto with zarith
+ end; ring.
+ eq_tac; auto with zarith.
+ rewrite Zmult_minus_distr_l; rewrite <- H5; auto with zarith.
+ ring.
+ Qed.
+
+ Lemma _square_mod_wf_spec: forall w, _wf w ->
+   _wf (_square_mod w).
+ intros w2 H.
+ unfold _wf; rewrite _square_mod_spec; auto.
+ case (Z_mod_lt ([|w2|] * [|w2|]) [|b|]); auto with zarith.
+ Qed.
+
+ Let _power_mod :=
    fix pow_mod (x:w) (p:positive) {struct p} : w :=
      match p with
      | xH => x
@@ -159,12 +955,96 @@ Section Mod_op.
        _mul_mod (_square_mod pow) x
      end.
 
+ Lemma _power_mod_spec: forall w p, _wf w ->
+   [|_power_mod w p|] = (Zpower_pos [|w|] p) mod [|b|].
+ assert(aux: forall w p, _wf w ->
+   [|_power_mod w p|] = (Zpower_pos [|w|] p) mod [|b|] /\ _wf (_power_mod w p)).
+ intros w2 p; elim p; simpl; auto with zarith.
+ intros p' Rec H. 
+ case (Rec H); intros Rec1 Rec2; clear Rec.
+ match goal with |- ?A /\ ?B =>
+   assert A; try (split; auto)
+ end.
+ replace (xI p') with (p' + p' + 1)%positive.
+ repeat rewrite Zpower_pos_is_exp; auto with zarith.
+ rewrite _mul_mod_spec; auto with zarith.
+ rewrite _square_mod_spec; auto with zarith.
+ rewrite Rec1; auto with zarith.
+ assert (tmp: forall p, Zpower_pos p 1 = p); try (rewrite tmp; clear tmp).
+ intros p1; unfold Zpower_pos; simpl; ring.
+ rewrite <- Zmod_mult; auto with zarith.
+ rewrite Zmod_mult; auto with zarith.
+ rewrite Zmod_mod; auto with zarith.
+ rewrite <- Zmod_mult; auto with zarith.
+ apply _square_mod_wf_spec; auto.
+ rewrite xI_succ_xO; rewrite <- Pplus_diag.
+ rewrite Pplus_one_succ_r; auto.
+ apply _mul_mod_wf_spec; auto with zarith.
+ apply _square_mod_wf_spec; auto with zarith.
+ intros p' Rec H. 
+ case (Rec H); intros Rec1 Rec2; clear Rec.
+ match goal with |- ?A /\ ?B =>
+   assert A; try (split; auto)
+ end.
+ replace (xO p') with (p' + p')%positive.
+ repeat rewrite Zpower_pos_is_exp; auto with zarith.
+ rewrite _square_mod_spec; auto with zarith.
+ rewrite Rec1; auto with zarith.
+ rewrite <- Zmod_mult; auto with zarith.
+ rewrite <- Pplus_diag; auto.
+ apply _square_mod_wf_spec; auto with zarith.
+ intros H; split; auto.
+ assert (tmp: forall p, Zpower_pos p 1 = p); try (rewrite tmp; clear tmp).
+ intros p1; unfold Zpower_pos; simpl; ring.
+ red in H; rewrite Zmod_def_small; auto with zarith.
+ case (spec_to_Z op_spec w2); auto with zarith.
+ intros w2 p H; case (aux w2 p); auto.
+ Qed.
+
+ Lemma _power_mod_wf_spec: forall w p, _wf w ->
+   _wf (_power_mod w p).
+ intros w2 p H.
+ unfold _wf; rewrite _power_mod_spec; auto.
+ case (Z_mod_lt (Zpower_pos [|w2|] p) [|b|]); auto with zarith.
+ Qed.
+
+(*
+      shift_spec        :
+              forall w p, wf w -> 
+                          [|shift m_op w p|] = ([|w|] / (Zpower_pos 2 p)) mod [|b|];
+      trunc_spec        :
+              forall w p, wf w ->
+                          [|power_mod m_op w p|] = ([|w1|] mod (Zpower_pos 2 p)) mod [|b|]
+*)
+
  Definition make_mod_op := 
    mk_mod_op
      _w0_mod _w1_mod 
      _succ_mod _add_mod 
      _pred_mod _sub_mod
      _mul_mod _square_mod _power_mod.
+
+  Definition new_mod_spec: mod_spec make_mod_op _wf.
+  apply mk_mod_spec.
+  exact _w0_wf.
+  exact _w1_wf.
+  exact _succ_mod_wf_spec.
+  exact _add_mod_wf_spec.
+  exact _pred_mod_wf_spec.
+  exact _sub_mod_wf_spec.
+  exact _mul_mod_wf_spec.
+  exact _square_mod_wf_spec.
+  exact _power_mod_wf_spec.
+  rewrite _w0_is_0; apply Zmod_def_small; auto with zarith.
+  rewrite _w1_is_1; apply Zmod_def_small; auto with zarith.
+  exact _succ_mod_spec.
+  exact _add_mod_spec.
+  exact _pred_mod_spec.
+  exact _sub_mod_spec.
+  exact _mul_mod_spec.
+  exact _square_mod_spec.
+  exact _power_mod_spec.
+  Defined.
 
 End Mod_op.
     
